committing bfs with imp implementation

bfs.v
@@ -1,6 +1,7 @@
 (*Authors: Syed Mohammed Arshad Zaidi, Anuj Sharma*)
 
 Require Import Coq.Lists.List.
+Require Import Coq.omega.Omega.
 
 (* This is representation of single node of a graph *)
 Inductive node :=
@@ -51,12 +52,367 @@ Definition nodes_equal a b :=
  
  Definition customNode := Node 1.
  Definition noCustomNode := Node 404.
- Definition customGraph := [(Node 1, [Node 2; Node 3]);(Node 2, [Node 3;Node 4])].
+ Definition customGraph := [(Node 1, [Node 2; Node 3]);(Node 2, [Node 4;Node 5]); (Node 3, [Node 6; Node 7]);(Node 4, [Node 8; Node 9])].
  
  Check customGraph.
  
  Compute (search_node customGraph (Node 2)).
+
+ Compute (is_node_present customGraph [] (Node 2)).
  
  Compute (nodes_equal (Node 2) (Node 4)).
  
  Compute (is_node_present customGraph [] customNode).
+
+ (* This function will remove node from graph which is passed. *)
+ Fixpoint remove_node (g: list(node*(list node))) (r: node) : list(node*(list node)) :=
+   match g with
+   | [] => []
+   | h::t => match h with
+             | (x,y) => match nodes_equal x r with
+                        | true => t
+                        | false => h::(remove_node t r)
+                        end
+             end
+   end.
+
+ Fixpoint remove_node_list (l: list node) (n: node) : list node :=
+   match l with
+   | [] => []
+   | h::t => match nodes_equal n h with
+             | true => remove_node_list t n
+             | false => h::(remove_node_list t n)
+             end
+   end.
+
+ (* Function for bfs traversal of custom graph. *)
+ (* Fixpoint bfs (g:list(node*(list node))) (s:list node) : list node :=
+   match s with
+   | [] => []
+   | h::t => h::(bfs g (t ++ (is_node_present g [] h)))
+   end.
+  *)
+
+ Inductive id : Type :=
+ | Id : nat -> id.
+
+ Definition beq_id id1 id2 :=
+  match id1,id2 with
+    | Id n1, Id n2 => beq_nat n1 n2
+  end.
+
+ Definition total_map (A:Type) := id -> A.
+
+ Definition t_empty {A:Type} (v : A) : total_map A :=
+   (fun _ => v).
+
+ Definition t_update {A:Type} (m : total_map A)
+                    (x : id) (v : A) :=
+  fun x' => if beq_id x x' then v else m x'.
+ 
+Inductive aexp : Type :=
+  | ANum : nat -> aexp
+  | AId : id -> aexp                (* <----- NEW *)
+  | APlus : aexp -> aexp -> aexp
+  | AMinus : aexp -> aexp -> aexp
+  | AMult : aexp -> aexp -> aexp.
+
+ 
+Inductive bexp : Type :=
+  | BTrue : bexp
+  | BFalse : bexp
+  | BEq : aexp -> aexp -> bexp
+  | BLe : aexp -> aexp -> bexp
+  | BNot : bexp -> bexp
+  | BAnd : bexp -> bexp -> bexp.
+
+
+Inductive com : Type :=
+  | CSkip : com
+  | CAss : id -> aexp -> com
+  | CSeq : com -> com -> com
+  | CIf : bexp -> com -> com -> com
+  | CWhile : bexp -> com -> com.
+
+Notation "'SKIP'" :=
+  CSkip.
+Notation "x '::=' a" :=
+  (CAss x a) (at level 60).
+Notation "c1 ;; c2" :=
+  (CSeq c1 c2) (at level 80, right associativity).
+Notation "'WHILE' b 'DO' c 'END'" :=
+  (CWhile b c) (at level 80, right associativity).
+Notation "'IFB' c1 'THEN' c2 'ELSE' c3 'FI'" :=
+  (CIf c1 c2 c3) (at level 80, right associativity).
+
+(* Function for bfs traversal of custom graph. *)
+ (* Fixpoint bfs (g:list(node*(list node))) (s:list node) : list node :=
+   match s with
+   | [] => []
+   | h::t => h::(bfs g (t ++ (is_node_present g [] h)))
+   end.
+  *)
+
+Definition state := total_map nat.
+
+Definition empty_state : state :=
+  t_empty 0.
+
+Fixpoint aeval (st : state) (a : aexp) : nat :=
+  match a with
+  | ANum n => n
+  | AId x => st x                                (* <----- NEW *)
+  | APlus a1 a2 => (aeval st a1) + (aeval st a2)
+  | AMinus a1 a2  => (aeval st a1) - (aeval st a2)
+  | AMult a1 a2 => (aeval st a1) * (aeval st a2)
+  end.
+
+Fixpoint beval (st : state) (b : bexp) : bool :=
+  match b with
+  | BTrue       => true
+  | BFalse      => false
+  | BEq a1 a2   => beq_nat (aeval st a1) (aeval st a2)
+  | BLe a1 a2   => leb (aeval st a1) (aeval st a2)
+  | BNot b1     => negb (beval st b1)
+  | BAnd b1 b2  => andb (beval st b1) (beval st b2)
+  end.
+
+Reserved Notation "e '\\' n" (at level 50, left associativity).
+
+Inductive aevalR : aexp -> nat -> Prop :=
+  | E_ANum : forall (n:nat),
+      (ANum n) \\ n
+  | E_APlus : forall (e1 e2: aexp) (n1 n2 : nat),
+      (e1 \\ n1) -> (e2 \\ n2) -> (APlus e1 e2) \\ (n1 + n2)
+  | E_AMinus : forall (e1 e2: aexp) (n1 n2 : nat),
+      (e1 \\ n1) -> (e2 \\ n2) -> (AMinus e1 e2) \\ (n1 - n2)
+  | E_AMult :  forall (e1 e2: aexp) (n1 n2 : nat),
+      (e1 \\ n1) -> (e2 \\ n2) -> (AMult e1 e2) \\ (n1 * n2)
+
+  where "e '\\' n" := (aevalR e n) : type_scope.
+
+Reserved Notation "c1 '/' st '\\' st'"
+                  (at level 40, st at level 39).
+
+Inductive ceval : com -> state -> state -> Prop :=
+  | E_Skip : forall st,
+      SKIP / st \\ st
+  | E_Ass  : forall st a1 n x,
+      aeval st a1 = n ->
+      (x ::= a1) / st \\ (t_update st x n)
+  | E_Seq : forall c1 c2 st st' st'',
+      c1 / st  \\ st' ->
+      c2 / st' \\ st'' ->
+      (c1 ;; c2) / st \\ st''
+  | E_IfTrue : forall st st' b c1 c2,
+      beval st b = true ->
+      c1 / st \\ st' ->
+      (IFB b THEN c1 ELSE c2 FI) / st \\ st'
+  | E_IfFalse : forall st st' b c1 c2,
+      beval st b = false ->
+      c2 / st \\ st' ->
+      (IFB b THEN c1 ELSE c2 FI) / st \\ st'
+  | E_WhileEnd : forall b st c,
+      beval st b = false ->
+      (WHILE b DO c END) / st \\ st
+  | E_WhileLoop : forall st st' st'' b c,
+      beval st b = true ->
+      c / st \\ st' ->
+      (WHILE b DO c END) / st' \\ st'' ->
+      (WHILE b DO c END) / st \\ st''
+
+  where "c1 '/' st '\\' st'" := (ceval c1 st st').
+
+
+Definition X : id := Id 5.
+Definition Y : id := Id 1.
+Definition Z : id := Id 2.
+
+Definition fact_in_coq : com :=
+  Z ::= AId X;;
+  Y ::= ANum 1;;
+  WHILE BNot (BEq (AId Z) (ANum 0)) DO
+    Y ::= AMult (AId Y) (AId Z);;
+    Z ::= AMinus (AId Z) (ANum 1)
+    END.
+
+Definition fact_in_coq' : com :=
+  Y ::= ANum 1;;
+  Z ::= ANum 3;;
+ 
+  WHILE BNot (BEq (AId Z) (ANum 0)) DO
+    Y ::= AMult (AId Y) (AId Z);;
+    Z ::= AMinus (AId Z) (ANum 1)
+    END.
+
+
+Compute t_update (t_update (t_update empty_state X 2) Z 0) Y 2.
+Compute t_update empty_state X 2.
+
+(*
+(X ::= ANum 2) / empty_state \\ t_update empty_state X 2
+*)
+
+Example test_fact: fact_in_coq'
+   / empty_state
+   \\ (t_update(t_update(t_update(t_update(t_update(t_update(t_update(t_update empty_state Y 1) Z 3) Y 3) Z 2) Y 6) Z 1) Y 6) Z 0).
+Proof.
+  unfold fact_in_coq'.
+  apply E_Seq with (t_update empty_state Y 1).
+  - apply E_Ass. reflexivity.
+  - apply E_Seq with (t_update (t_update empty_state Y 1) Z 3).
+    + apply E_Ass. reflexivity.
+    + apply E_WhileLoop with (t_update(t_update(t_update(t_update empty_state Y 1) Z 3) Y 3) Z 2).
+      * reflexivity.
+      * apply E_Seq with (t_update(t_update (t_update empty_state Y 1) Z 3) Y 3).
+        { apply E_Ass. reflexivity. }
+        { apply E_Ass. reflexivity. }
+      * apply E_WhileLoop with (t_update(t_update(t_update(t_update(t_update(t_update empty_state Y 1) Z 3) Y 3) Z 2) Y 6) Z 1).
+        { reflexivity. }
+        { apply E_Seq with (t_update(t_update(t_update(t_update(t_update empty_state Y 1) Z 3) Y 3) Z 2) Y 6).
+          { apply E_Ass. reflexivity. }
+          { apply E_Ass. reflexivity. }
+        }
+        { apply E_WhileLoop with (t_update(t_update(t_update(t_update(t_update(t_update(t_update(t_update empty_state Y 1) Z 3) Y 3) Z 2) Y 6) Z 1) Y 6) Z 0).
+          { reflexivity. }
+          { apply E_Seq with (t_update(t_update(t_update(t_update(t_update(t_update(t_update empty_state Y 1) Z 3) Y 3) Z 2) Y 6) Z 1) Y 6).
+            { apply E_Ass. reflexivity. }
+            { apply E_Ass. reflexivity. } }
+          { apply E_WhileEnd. simpl. reflexivity. } }
+Qed.
+
+            
+ Compute is_node_present customGraph [] (Node 4).
+
+ (* Compute bfs customGraph [Node 1].*)
+
+ Fixpoint graph_to_list (g: list(node*(list node))) : list node :=
+   match g with
+   | [] => []
+   | h::t => match h with
+             | (x,y) => [x] ++ y ++ (graph_to_list t)
+             end
+   end.
+
+ Fixpoint node_in_list (l: list node) (n: node) : bool :=
+   match l with
+   | [] => false
+   | h::t => match nodes_equal h n with
+             | true => true
+             | false => node_in_list t n
+             end
+   end.
+
+ Compute remove_node_list (graph_to_list customGraph) (Node 3).
+ Compute node_in_list (graph_to_list customGraph) (Node 21).
+ Check [Node 1] ++ [(Node 2); (Node 3)].
+
+ Fixpoint unique_list (r: list node) (l: list node) : list node :=
+   match l with
+   | [] => r
+   | h::t => match node_in_list r h with
+             | false => unique_list (r ++ [h]) t
+             | true => unique_list r t
+             end
+   end.
+
+ Compute graph_to_list customGraph.
+ Compute unique_list [] (graph_to_list customGraph).
+
+ Definition removed_one := remove are_nodes_equal (Node 1) (unique_list [] (graph_to_list customGraph)).
+ Definition removed_two := remove are_nodes_equal (Node 2) removed_one.
+ Compute removed_two.
+ Definition removed_three := remove are_nodes_equal (Node 3) removed_two.
+ Definition removed_four := remove are_nodes_equal (Node 4) removed_three.
+ Compute removed_four.
+
+ (* Following lemma will state for removal of nodes in each iteration of bfs which results in termination of bfs traversal. *)
+ Lemma bfs_iteration_custom : forall nd grph_nodes,
+  length grph_nodes >= length (remove are_nodes_equal nd grph_nodes) /\
+  (In nd grph_nodes -> length grph_nodes > length (remove are_nodes_equal nd grph_nodes)).
+Proof.
+  intros; induction grph_nodes; split; intros; simpl; try (omega).
+  - inversion H.
+  - simpl. destruct IHgrph_nodes as [H1 H2].
+  remember (are_nodes_equal nd a) as visited_a. destruct visited_a; simpl; omega.
+  - simpl. destruct IHgrph_nodes as [H1 H2].
+    + destruct H as [H3 | H4]. remember (are_nodes_equal nd a) as visited_a. destruct visited_a; simpl.
+      * omega.
+      * subst. destruct n.
+        { reflexivity. }
+      * remember (are_nodes_equal nd a) as visited_a. destruct visited_a; simpl.
+        { omega. }
+        { remember (H2 H4) as H5. omega. }
+Qed.
+
+(* Defining notation for cons *)
+Notation "x :: l" := (cons x l).
+
+
+Inductive bfs_ind : graph -> list node -> Prop :=
+| bfs_empty : bfs_ind [] []
+| bfs_single : forall n, bfs_ind [(n,[])] [n]
+| bfs_list_s: forall g n l l' n', bfs_ind [(n,l');g] l -> bfs_ind [(n',[n]);(n,l');g] (n':: l).
+
+Definition inputGraph := [(Node 1, [Node 2; Node 3]);(Node 2, [Node 4;Node 5]); (Node 3, [Node 6; Node 7]);(Node 4, [Node 8; Node 9])].
+
+(* This will hold all vertices of current iteration. *)
+(* Initializing it with starting vertex. *)
+Definition current_stack := [Node 1].
+
+(* Function to check if our node list is empty or not. *)
+Definition not_empty (l: list node) : bexp :=
+  match l with
+    |[] => BTrue
+    | _ => BFalse
+  end.
+
+Definition get_next_node :=
+  match current_stack with
+  | [] => []
+  | h::t => [h]
+  end.
+
+Definition get_next_node_num :=
+  match current_stack with
+  | [] => (ANum 0)
+  | h::t => match h with
+            | (Node x) => (ANum x)
+            end
+  end.
+
+Definition process_iteration (l: list node) : aexp :=
+  get_next_node_num.
+
+Definition pop :=
+  match current_stack with
+  | [] => []
+  | h::t => t
+  end.
+
+Definition get_adj_nodes (x: aexp) : list(node) :=
+  match x with
+  | (ANum y) => (is_node_present inputGraph [] (Node y))
+  | _        => []
+  end.
+
+Definition bfs_iteration :=
+  Y ::= process_iteration(current_stack ++ get_adj_nodes(get_next_node_num)).
+
+Definition bfs : com :=
+    Y ::= ANum 1;;
+    
+    WHILE BNot (BEq (AId Y) (ANum 0)) DO
+    bfs_iteration
+    END.
+
+Example test_bfs :
+  bfs / empty_state \\ (t_update(t_update empty_state Y 1)Y 1).
+Proof.
+  unfold bfs.
+  apply E_Seq with (t_update empty_state Y 1).
+  - apply E_Ass. simpl. reflexivity.
+  - apply E_WhileLoop with (t_update(t_update empty_state Y 1)Y 1).
+    + simpl. reflexivity.
+    + unfold bfs_iteration. apply E_Ass. simpl. reflexivity.
+    + (* this will be done once our current_stack start reducing *)
